iris_system/algebra/functions.v
@@ -1,0 +1,18 @@
+(* functions.v with auxiliary lemmas *)
+From iris.algebra Require Export functions.
+Require Import sflib.
+
+Section cmra.
+  Context {A : Type} `{Heqdec : !EqDecision A} {B : A → ucmra}.
+  Implicit Types x y : A.
+  Implicit Types f g h : discrete_fun B.
+
+  Lemma discrete_fun_delete i f :
+    f ≡ (((λ x, if (decide (x = i)) then ε else (f x)) : discrete_fun B)
+        ⋅ (discrete_fun_singleton i (f i)) : discrete_fun B).
+  Proof.
+    intros x; rewrite discrete_fun_lookup_op; des_ifs; first by rewrite discrete_fun_lookup_singleton left_id.
+    rewrite discrete_fun_lookup_singleton_ne; first by rewrite (comm op) left_id.
+    ii; clarify.
+  Qed.
+End cmra.
